\documentclass[a4paper,12pt]{article}

\usepackage{times}
\usepackage{amsmath}

\newcommand{\D}{\mathrm{d}}
\newcommand{\E}{\mathrm{e}}
\newcommand{\J}{\mathrm{i}}

\bibliographystyle{unsrt}

\begin{document}

Notes and derivations not given explicitly in referenced documents.

Derivatives of regular Laplace expansions, assuming normalized
Legendre functions and unit normalization constants ($\alpha$ and
$\beta$ in G\&D). Identities for Legendre functions come from
CS-TR-4264. 

\begin{align}
  \partial_{z} &= \mu\frac{\partial}{\partial r}
  + \frac{1-\mu^{2}}{r}\frac{\partial}{\partial \mu},\\
  \partial_{xy} &= \frac{\partial}{\partial x} + \J
  \frac{\partial}{\partial y}\\
  &=
  \frac{\E^{\J\phi}}{r(1-\mu^{2})^{1/2}}
  \left[
    (1-\mu^{2})
    \left(
      r\frac{\partial}{\partial r}
      -\mu\frac{\partial}{\partial \mu}
    \right)
    + \J\frac{\partial}{\partial \phi}
  \right],\\
  \overline{\partial_{xy}}
  &= \frac{\partial}{\partial x} - \J
  \frac{\partial}{\partial y}\\
  &=
  \frac{\E^{-\J\phi}}{r(1-\mu^{2})^{1/2}}
  \left[
    (1-\mu^{2})
    \left(
      r\frac{\partial}{\partial r}
      -\mu\frac{\partial}{\partial \mu}
    \right)
    - \J\frac{\partial}{\partial \phi}
  \right],\\
  \partial_{x} &= (\partial_{xy}+\overline{\partial_{xy}})/2,\\
  \partial_{y} &= -\J(\partial_{xy}-\overline{\partial_{xy}})/2.
\end{align}

\begin{align}
  R_{n}^{m} &= r^{n} N_{n}^{m}P_{n}^{|m|}\E^{\J m \phi},\\
  \frac{\partial R_{n}^{m}}{\partial z}
  &=
  \left[
    \mu n r^{n-1}P_{n}^{|m|} + r^{n-1}(1-\mu^{2})
    \frac{\partial P_{n}^{|m|}}{\partial \mu}
  \right]\E^{\J m \phi} N_{n}^{m},\\
  &= r^{n-1}N_{n}^{m}P_{n-1}^{|m|}\E^{\J m \phi},\\
  &= \frac{N_{n}^{m}}{N_{n-1}^{m}}R_{n-1}^{m},\\
  &=
  \left[
    \frac{2n+1}{2n-1}
    (n^{2}-m^{2})
  \right]^{1/2}R_{n-1}^{m}.
\end{align}

\begin{align}
  S_{n}^{m} &= r^{-n-1}N_{n}^{m}P_{n}^{|m|}\E^{\J m\phi},\\
  \partial_{z} S_{n}^{m}
  &=
  -\left[
    \mu (n+1) r^{-n-2}P_{n}^{|m|} + r^{-n-2}(1-\mu^{2})
    \frac{\partial P_{n}^{|m|}}{\partial \mu}
  \right]\E^{\J m \phi} N_{n}^{m},\\
  &= -r^{-n-2}N_{n}^{m}(n-|m|+1)P_{n+1}^{|m|}\E^{\J m \phi},\\
  &= -(n-|m|+1)\frac{N_{n}^{m}}{N_{n+1}^{m}}S_{n+1}^{m},\\
  &=
  -\left\{
    \frac{2n+1}{2n+3}
    \left[(n+1)^{2}-m^{2}\right]
  \right\}^{1/2}S_{n+1}^{m},\\
  \partial_{xy}S_{n}^{m}
  &= 
  \biggl\{
  \left(1-\mu^{2}\right)^{1/2}
  \left[
    -(n+1)P_{n}^{|m|}(\mu)
    -\mu\frac{\partial P_{n}^{|m|}}{\partial \mu}
  \right]-\nonumber\\
  &\frac{m}{\left(1-\mu^{2}\right)^{1/2}}
  P_{n}^{|m|}(\mu)
  \biggr\}N_{n}^{m}\E^{\J(m+1)\phi}r^{-n-2},\\
  &= \left[
    \frac{2n+1}{2n+3}(n+m+1)(n+m+2)
  \right]^{1/2}S_{n+1}^{m+1},\\
  \overline{\partial_{xy}}S_{n}^{m}
  &= 
  \biggl\{
  \left(1-\mu^{2}\right)^{1/2}
  \left[
    -(n+1)P_{n}^{|m|}(\mu)
    -\mu\frac{\partial P_{n}^{|m|}}{\partial \mu}
  \right]+\nonumber\\
  &\frac{m}{\left(1-\mu^{2}\right)^{1/2}}
  P_{n}^{|m|}(\mu)
  \biggr\}N_{n}^{m}\E^{\J(m-1)\phi}r^{-n-2},\\
  &= -\left[
    \frac{2n+1}{2n+3}(n-m+1)(n-m+2)
  \right]^{1/2}S_{n+1}^{m-1}.
\end{align}

We store rotation coefficients $H_{n}^{\nu m}$ for $\nu=-n,\ldots,n$,
$m=0,\ldots,n$. By symmetry (G\&D 5.5.2):
\begin{align*}
  H_{n}^{\nu, -m} &= H_{n}^{-\nu, m}.
\end{align*}

\nocite{gumerov-duraiswami03}

\bibliography{abbrev,maths}

\end{document}

%%% Local Variables:
%%% mode: latex
%%% TeX-master: t
%%% End:
